Separate Arity consistency from Cardinality consistency

Launchbury/ArityEtaExpandCorrect.thy
@@ -1,16 +1,16 @@
 theory ArityEtaExpandCorrect
-imports ArityEtaExpand  ArityAnalysisSpec ArityEtaExpansionSestoft AbstractTransform ConstOn
+imports ArityEtaExpand ArityConsistent ArityAnalysisSpec ArityEtaExpansionSestoft AbstractTransform ConstOn
 begin
 
 locale CardinalityArityTransformation = CorrectArityAnalysisLetNoCard
 begin
-
   sublocale AbstractTransformBoundSubst
     "\<lambda> a . inc\<cdot>a"
     "\<lambda> a . pred\<cdot>a"
     "\<lambda> \<Delta> e a . (a, Aheap \<Delta> e\<cdot>a)"
     "fst"
     "snd"
+    "\<lambda> _. 0"
     "Aeta_expand"
     "snd"
   apply default
@@ -18,7 +18,7 @@ begin
   apply (rule subst_Aeta_expand)
   done
 
-  abbreviation aTransform where "aTransform \<equiv> transform"
+  abbreviation ccTransform where "ccTransform \<equiv> transform"
 
   lemma supp_transform: "supp (transform a e) \<subseteq> supp e"
     by (induction rule: transform.induct)
@@ -26,249 +26,251 @@ begin
   interpretation supp_bounded_transform transform
     by default (auto simp add: fresh_def supp_transform) 
 
-  fun conf_transform :: "(AEnv \<times> Arity) \<Rightarrow> conf \<Rightarrow> conf"
-  where "conf_transform (ae,  a) (\<Gamma>, e, S) =
-    (map_transform Aeta_expand ae (map_transform transform ae \<Gamma>), 
-     transform a e,
-     S)"
+  fun transform_alts :: "Arity list \<Rightarrow> stack \<Rightarrow> stack"
+    where 
+      "transform_alts _ [] = []"
+    | "transform_alts (a#as) (Alts e1 e2 # S) = (Alts (ccTransform a e1) (ccTransform a e2)) # transform_alts as S"
+    | "transform_alts as (x # S) = x # transform_alts as S"
 
-  inductive consistent :: "(AEnv \<times> Arity) \<Rightarrow> conf \<Rightarrow> bool" where
+  lemma transform_alts_Nil[simp]: "transform_alts [] S = S"
+    by (induction  S) auto
+
+  lemma Astack_transform_alts[simp]:
+    "Astack (transform_alts as S) = Astack S"
+   by (induction rule: transform_alts.induct) auto
+
+  lemma fresh_star_transform_alts[intro]: "a \<sharp>* S \<Longrightarrow> a \<sharp>* transform_alts as S"
+   by (induction as S  rule: transform_alts.induct) (auto simp add: fresh_star_Cons)
+
+  fun a_transform :: "astate \<Rightarrow> conf \<Rightarrow> conf"
+  where "a_transform (ae, a, as) (\<Gamma>, e, S) =
+    (map_transform Aeta_expand ae (map_transform ccTransform ae \<Gamma>), 
+     ccTransform a e,
+     transform_alts as  S)"
+
+  fun restr_conf :: "var set \<Rightarrow> conf \<Rightarrow> conf"
+    where "restr_conf V (\<Gamma>, e, S) = (restrictA V \<Gamma>, e, restr_stack V S)"
+
+  inductive consistent :: "astate \<Rightarrow> conf \<Rightarrow> bool" where
     consistentI[intro!]: 
-    "edom ae \<subseteq> domA \<Gamma> \<union> upds S
+    "a_consistent (ae, a, as) (\<Gamma>, e, S)
     \<Longrightarrow> heap_upds_ok (\<Gamma>, S)
-    \<Longrightarrow> Astack S \<sqsubseteq> a
-    \<Longrightarrow> ABinds \<Gamma>\<cdot>ae \<squnion> Aexp e\<cdot>a \<sqsubseteq> ae
-    \<Longrightarrow> const_on ae (thunks \<Gamma>) (up\<cdot>0)
-    \<Longrightarrow> const_on ae (ap S) (up\<cdot>0)
-    \<Longrightarrow> const_on ae (upds S) (up\<cdot>0)
-    \<Longrightarrow> consistent (ae, a) (\<Gamma>, e, S)"  
-  inductive_cases consistentE[elim!]: "consistent (ae, a) (\<Gamma>, e, S)"
-  
+    \<Longrightarrow> (\<And> x. x \<in> thunks \<Gamma> \<Longrightarrow>  ae x = up\<cdot>0)
+    \<Longrightarrow> consistent (ae, a, as) (\<Gamma>, e, S)"  
+  inductive_cases consistentE[elim!]: "consistent (ae, a, as) (\<Gamma>, e, S)"
+
+  lemma closed_consistent:
+    assumes "fv e = ({}::var set)"
+    shows "consistent (\<bottom>, 0, []) ([], e, [])"
+  by (auto simp add: edom_empty_iff_bot closed_a_consistent[OF assms])
+
   lemma foo:
     fixes c c' R 
-    assumes "c \<Rightarrow>\<^sup>* c'" and "\<not> boring_step c'" and "consistent (ae,a) c"
-    shows "\<exists>ae' ce' a'. consistent (ae',a') c' \<and> conf_transform (ae,a) c \<Rightarrow>\<^sup>* conf_transform (ae',a') c'"
+    assumes "c \<Rightarrow>\<^sup>* c'" and "\<not> boring_step c'" and "consistent (ae,a,as) c"
+    shows "\<exists>ae' a' as'. consistent (ae',a',as') c' \<and> a_transform (ae,a,as) c \<Rightarrow>\<^sup>* a_transform (ae',a',as') c'"
   using assms
-  proof(induction c c' arbitrary: ae a rule:step_induction)
+  proof(induction c c' arbitrary: ae a as rule:step_induction)
   case (app\<^sub>1 \<Gamma> e x S)
-    from app\<^sub>1 have "consistent (ae, inc\<cdot>a) (\<Gamma>, e, Arg x # S)"
-      by (auto simp add: join_below_iff  dest!: below_trans[OF Aexp_App] elim: below_trans)
+    from app\<^sub>1 have "consistent (ae, inc\<cdot>a, as) (\<Gamma>, e, Arg x # S)"
+      by (auto intro: a_consistent_app\<^sub>1)
     moreover
-    have "conf_transform (ae, a) (\<Gamma>, App e x, S) \<Rightarrow> conf_transform (ae, inc\<cdot>a) (\<Gamma>, e, Arg x # S)"
+    have "a_transform (ae, a, as) (\<Gamma>, App e x, S) \<Rightarrow> a_transform (ae, inc\<cdot>a, as) (\<Gamma>, e, Arg x # S)"
       by simp rule
     ultimately
     show ?case by (blast del: consistentI consistentE)
   next
-case (app\<^sub>2 \<Gamma> y e x S)
-  {
-  have "Aexp (e[y::=x])\<cdot>(pred\<cdot>a) \<sqsubseteq> env_delete y ((Aexp e)\<cdot>(pred\<cdot>a)) \<squnion> esing x\<cdot>(up\<cdot>0)" by (rule Aexp_subst)
-  also have "env_delete y ((Aexp e)\<cdot>(pred\<cdot>a)) \<sqsubseteq> Aexp (Lam [y]. e)\<cdot>a" by (rule Aexp_Lam)
-  also have "\<dots> \<sqsubseteq> ae" using app\<^sub>2 by (auto simp add: join_below_iff)
-  also have "esing x\<cdot>(up\<cdot>0) \<sqsubseteq> ae" using app\<^sub>2 by auto
-  also have "ae \<squnion> ae = ae" by simp
-  finally  have "Aexp (e[y::=x])\<cdot>(pred\<cdot>a) \<sqsubseteq> ae" by this simp_all
-  }
-  then
-  have "consistent (ae, pred\<cdot>a) (\<Gamma>, e[y::=x], S)" using app\<^sub>2
-    by (auto elim: below_trans edom_mono  simp add: join_below_iff)
-  moreover
-  have "conf_transform (ae, a) (\<Gamma>, Lam [y]. e, Arg x # S) \<Rightarrow> conf_transform (ae, pred \<cdot> a) (\<Gamma>, e[y::=x], S)" by (simp add: subst_transform[symmetric]) rule
-  ultimately
-  show ?case by (blast  del: consistentI consistentE)
-next
-case (thunk \<Gamma> x e S)
-  hence "x \<in> thunks \<Gamma>" by auto
-  hence [simp]: "x \<in> domA \<Gamma>" by (rule set_mp[OF thunks_domA])
-  hence "x \<notin> upds S" using thunk by (auto elim!: heap_upds_okE)
-
-  from thunk have "Aexp (Var x)\<cdot>a \<sqsubseteq> ae" by (auto simp add: join_below_iff)
-  from below_trans[OF Aexp_Var fun_belowD[OF this] ]
-  have "up\<cdot>a \<sqsubseteq> ae x".    
-  then obtain u where "ae x = up\<cdot>u" and "a \<sqsubseteq> u" by (cases "ae x") auto
-  hence [simp]: "x \<in> edom ae" by (simp add: edom_def)
-
-  have "ae x = up\<cdot>0" using thunk `x \<in> thunks \<Gamma>` by (auto)
-  hence "u = 0" using `ae x = up\<cdot>u` by simp
-
+  case (app\<^sub>2 \<Gamma> y e x S)
+    have "consistent (ae, pred\<cdot>a, as) (\<Gamma>, e[y::=x], S)" using app\<^sub>2
+      by (auto 4 3 intro: a_consistent_app\<^sub>2)
+    moreover
+    have "a_transform (ae, a, as) (\<Gamma>, Lam [y]. e, Arg x # S) \<Rightarrow> a_transform (ae, pred \<cdot> a, as) (\<Gamma>, e[y::=x], S)" by (simp add: subst_transform[symmetric]) rule
+    ultimately
+    show ?case by (blast  del: consistentI consistentE)
+  next
+  case (thunk \<Gamma> x e S)
+    hence "x \<in> thunks \<Gamma>" by auto
+    hence [simp]: "x \<in> domA \<Gamma>" by (rule set_mp[OF thunks_domA])
+    hence "x \<notin> upds S" using thunk by (auto elim!: heap_upds_okE)
+    
+    have "x \<in> edom ae" using thunk by auto
   
-  from Abinds_reorder1[OF `map_of \<Gamma> x = Some e`] `ae x = up\<cdot>u`
-  have "ABinds (delete x \<Gamma>)\<cdot>ae \<squnion> Aexp e\<cdot>u = ABinds \<Gamma>\<cdot>ae" by auto
-  also have "\<dots> \<sqsubseteq> ae" using thunk by (auto simp add: join_below_iff)
-  finally have "ABinds (delete x \<Gamma>)\<cdot>ae \<squnion> Aexp e\<cdot>u \<sqsubseteq> ae".
-  hence "consistent (ae, 0) (delete x \<Gamma>, e, Upd x # S)" using thunk `ae x = up\<cdot>u` `u = 0`
-    by (auto intro!: const_onI)
-  moreover
+    have "ae x = up\<cdot>0" using thunk `x \<in> thunks \<Gamma>` by (auto)
 
-  from  `map_of \<Gamma> x = Some e` `ae x = up\<cdot>0`
-  have "map_of (map_transform Aeta_expand ae (map_transform transform ae \<Gamma>)) x = Some (transform 0 e)"
-    by (simp add: map_of_map_transform)
-  with `\<not> isVal e`
-  have "conf_transform (ae, a) (\<Gamma>, Var x, S) \<Rightarrow> conf_transform (ae, 0) (delete x \<Gamma>, e, Upd x # S)"
-    by (auto simp add: map_transform_delete restr_delete_twist intro!: step.intros  simp del: restr_delete)
-  ultimately
-  show ?case by (blast del: consistentI consistentE)
-next
-case (lamvar \<Gamma> x e S)
-  from lamvar have [simp]: "x \<in> domA \<Gamma>" by auto (metis domI dom_map_of_conv_domA)
-  from lamvar have "Aexp (Var x)\<cdot>a \<sqsubseteq> ae" by (auto simp add: join_below_iff)
-  from below_trans[OF Aexp_Var fun_belowD[OF this] ]
-  have "up\<cdot>a \<sqsubseteq> ae x".
-  then obtain u where "ae x = up\<cdot>u" and "a \<sqsubseteq> u" by (cases "ae x") auto
+    have "a_consistent (ae, 0, as) (delete x \<Gamma>, e, Upd x # S)" using thunk `ae x = up\<cdot>0`
+      by (auto intro!: a_consistent_thunk_0 simp del: restr_delete)
+    hence "consistent (ae, 0, as) (delete x \<Gamma>, e, Upd x # S)" using thunk `ae x = up\<cdot>0` 
+      by (auto simp add:  restr_delete_twist)
+    moreover
+  
+    from  `map_of \<Gamma> x = Some e` `ae x = up\<cdot>0`
+    have "map_of (map_transform Aeta_expand ae (map_transform ccTransform ae \<Gamma>)) x = Some (transform 0 e)"
+      by (simp add: map_of_map_transform)
+    with `\<not> isVal e`
+    have "a_transform (ae, a, as) (\<Gamma>, Var x, S) \<Rightarrow> a_transform (ae, 0, as) (delete x \<Gamma>, e, Upd x # S)"
+      by (auto simp add: map_transform_delete restr_delete_twist intro!: step.intros  simp del: restr_delete)
+    ultimately
+    show ?case by (blast del: consistentI consistentE)
+  next
+  case (lamvar \<Gamma> x e S)
+    from lamvar(1) have [simp]: "x \<in> domA \<Gamma>" by (metis domI dom_map_of_conv_domA)
 
-  from Abinds_reorder1[OF `map_of \<Gamma> x = Some e`] `ae x = up\<cdot>u`
-  have "ABinds (delete x \<Gamma>)\<cdot>ae \<squnion> Aexp e\<cdot>u = ABinds \<Gamma>\<cdot>ae" by auto
-  also have "\<dots> \<sqsubseteq> ae" using lamvar by (auto simp add: join_below_iff)
-  finally have "ABinds (delete x \<Gamma>)\<cdot>ae \<squnion> Aexp e\<cdot>u \<sqsubseteq> ae".
+    have "up\<cdot>a \<sqsubseteq> (Aexp (Var x)\<cdot>a f|` (domA \<Gamma> \<union> upds S)) x"
+      by (simp) (rule Aexp_Var)
+    also from lamvar have "Aexp (Var x)\<cdot>a f|` (domA \<Gamma> \<union> upds S) \<sqsubseteq> ae" by (auto simp add: join_below_iff env_restr_join a_consistent.simps)
+    finally
+    obtain u where "ae x = up\<cdot>u" by (cases "ae x") (auto simp add: edom_def)
+    hence "x \<in> edom ae" by (auto simp add: edomIff)
 
-  have "consistent (ae, u) ((x, e) # delete x \<Gamma>, e, S)"
-    using lamvar `ABinds (delete x \<Gamma>)\<cdot>ae \<squnion> Aexp e\<cdot>u \<sqsubseteq> ae`  `ae x = up\<cdot>u` 
-    by (auto simp add: join_below_iff thunks_Cons split:if_splits intro: below_trans[OF _ `a \<sqsubseteq> u`] intro!: const_onI)
-  moreover
-
-  have "Astack S \<sqsubseteq> u" using lamvar  below_trans[OF _ `a \<sqsubseteq> u`] by auto
-
-  {
-  from `isVal e`
-  have "isVal (transform u e)" by simp
-  hence "isVal (Aeta_expand u (transform u e))" by (rule isVal_Aeta_expand)
-  moreover
-  from  `map_of \<Gamma> x = Some e`  `ae x = up \<cdot> u`  `isVal (transform u e)`
-  have "map_of (map_transform Aeta_expand ae (map_transform transform ae \<Gamma>)) x = Some (Aeta_expand u (transform u e))"
-    by (simp add: map_of_map_transform)
-  ultimately
-  have "conf_transform (ae, a) (\<Gamma>, Var x, S) \<Rightarrow>\<^sup>*
-        ((x, Aeta_expand u (transform u e)) # delete x (map_transform Aeta_expand ae (map_transform transform ae \<Gamma>)), Aeta_expand u  (transform u e), S)"
-     by (auto intro: lambda_var simp add: map_transform_delete simp del: restr_delete)
-  also have "\<dots> = ((map_transform Aeta_expand ae (map_transform transform ae ((x,e) # delete x \<Gamma>))), Aeta_expand u (transform u e), S)"
-    using `ae x = up \<cdot> u` `isVal (transform u e)`
-    by (simp add: map_transform_Cons map_transform_delete restr_delete_twist del: restr_delete)
-  also(subst[rotated]) have "\<dots> \<Rightarrow>\<^sup>* conf_transform (ae, u) ((x, e) # delete x \<Gamma>, e, S)"
-    by simp (rule Aeta_expand_correct[OF `Astack S \<sqsubseteq> u`])
-  finally(rtranclp_trans)
-  have "conf_transform (ae, a) (\<Gamma>, Var x, S) \<Rightarrow>\<^sup>* conf_transform (ae, u) ((x, e) # delete x \<Gamma>, e, S)".
-  }
-  ultimately show ?case by (blast del: consistentI consistentE)
-next
-case (var\<^sub>2 \<Gamma> x e S)
-
-  have "ae x = up\<cdot>a" using var\<^sub>2 by auto
-
-  have "Astack (Upd x # S) \<sqsubseteq> a" using var\<^sub>2 by auto
-  hence "a = 0" by auto
-
-  have "consistent (ae, 0) ((x, e) # \<Gamma>, e, S)" using var\<^sub>2
-    by (auto simp add: join_below_iff thunks_Cons split:if_splits)
-  moreover
-  have "conf_transform (ae, a) (\<Gamma>, e, Upd x # S) \<Rightarrow> conf_transform (ae, 0) ((x, e) # \<Gamma>, e, S)"
-    using `ae x = up\<cdot>a` `a = 0` var\<^sub>2
-    by (auto intro!: step.intros simp add: map_transform_Cons)
-  ultimately show ?case by (blast del: consistentI consistentE)
-next
-  case (let\<^sub>1 \<Delta> \<Gamma> e S)
-
-  let ?ae = "Aheap \<Delta> e\<cdot>a"
-  let ?new = "(domA (\<Delta> @ \<Gamma>) \<union> upds S - (domA \<Gamma> \<union> upds S))"
-  have new: "?new = domA \<Delta>"
-    using fresh_distinct[OF let\<^sub>1(1)] fresh_distinct_fv[OF let\<^sub>1(2)]
-    by (auto dest: set_mp[OF ups_fv_subset])
-
-  have "domA \<Delta> \<inter> upds S = {}" using fresh_distinct_fv[OF let\<^sub>1(2)] by (auto dest: set_mp[OF ups_fv_subset])
-  hence *: "\<And> x. x \<in> upds S \<Longrightarrow> x \<notin> edom ?ae" by (auto dest!: set_mp[OF edom_Aheap])
-
-  have restr_stack_simp: "restr_stack (edom (?ae \<squnion> ae)) S = restr_stack (edom ae) S"
-    by (auto intro: restr_stack_cong dest!: *)
-
-  have "edom ae \<subseteq> domA \<Gamma> \<union> upds S" using let\<^sub>1 by auto
-  from set_mp[OF this] fresh_distinct[OF let\<^sub>1(1)] fresh_distinct_fv[OF let\<^sub>1(2)]
-  have [simp]: "ae f|` domA \<Delta> = \<bottom>"
-    using  fresh_distinct[OF let\<^sub>1(1)] by (auto dest: set_mp[OF ups_fv_subset])
-
-  from  fresh_distinct[OF let\<^sub>1(1)]
-   have [simp]: "?ae f|` domA \<Gamma> = \<bottom>" by (auto dest!: set_mp[OF edom_Aheap])
-
-  {
-  have "edom (?ae \<squnion> ae) \<subseteq> domA (\<Delta> @ \<Gamma>) \<union> upds S"
-    using let\<^sub>1(3) by (auto dest: set_mp[OF edom_Aheap])
-  moreover
-  have "const_on (?ae \<squnion> ae) (thunks \<Gamma>) (up\<cdot>0)" using let\<^sub>1 by fastforce
-  moreover
-  { fix x e'
-    assume "x \<in> thunks \<Delta>" 
-    hence "x \<notin> domA \<Gamma>" and "x \<notin> upds S"
-      using fresh_distinct[OF let\<^sub>1(1)] fresh_distinct_fv[OF let\<^sub>1(2)]
-      by (auto dest!: set_mp[OF thunks_domA] set_mp[OF ups_fv_subset])
-    hence "(?ae \<squnion> ae) x = up \<cdot> 0" using `x \<in> thunks \<Delta>` by (auto simp add: Aheap_heap3)
-  }
-  hence "const_on (?ae \<squnion> ae) (thunks \<Delta>) (up\<cdot>0)" by auto
-  moreover
-  have "const_on ae (ap S) (up\<cdot>0)" using let\<^sub>1 by auto  
-  hence "const_on (?ae \<squnion> ae) (ap S) (up\<cdot>0)" by fastforce
-  moreover
-  have "const_on ae (upds S) (up\<cdot>0)" using let\<^sub>1 by auto
-  hence "const_on (?ae \<squnion> ae) (upds S) (up\<cdot>0)"  by fastforce
-  moreover
-  have "Astack S \<sqsubseteq> a" unfolding restr_stack_simp using let\<^sub>1 by auto
-  moreover
-  have "heap_upds_ok (\<Gamma>, S)" using let\<^sub>1 by auto
-  with fresh_distinct[OF let\<^sub>1(1)]  `domA \<Delta> \<inter> upds S = {}`
-  have "heap_upds_ok (\<Delta> @ \<Gamma>, S)" by (rule heap_upds_ok_append)
-  moreover
-  {
-  have "ABinds \<Delta>\<cdot>(Aheap \<Delta> e\<cdot>a \<squnion> ae) = ABinds \<Delta>\<cdot>(Aheap \<Delta> e\<cdot>a)"
-    by (rule Abinds_env_restr_cong) (simp add: env_restr_join)
-  moreover
-  have "ABinds \<Gamma>\<cdot>(Aheap \<Delta> e\<cdot>a \<squnion> ae) = ABinds \<Gamma>\<cdot>ae"
-    by (rule Abinds_env_restr_cong) (simp add: env_restr_join)
-  ultimately
-  have "ABinds (\<Delta> @ \<Gamma>) \<cdot> (Aheap \<Delta> e\<cdot>a \<squnion> ae) \<squnion> Aexp e\<cdot>a = (ABinds \<Delta>\<cdot>(Aheap \<Delta> e\<cdot>a) \<squnion> Aexp e\<cdot>a) \<squnion> ABinds \<Gamma>\<cdot>ae"
-    by (simp add: Abinds_append_disjoint[OF fresh_distinct[OF let\<^sub>1(1)]])
-  also have "\<dots> \<sqsubseteq> (Aheap \<Delta> e\<cdot>a \<squnion> Aexp (Let \<Delta> e)\<cdot>a) \<squnion> ABinds \<Gamma>\<cdot>ae" by (rule join_mono[OF Aexp_Let below_refl])
-  also have "\<dots> = Aheap \<Delta> e\<cdot>a \<squnion> (Aexp (Let \<Delta> e)\<cdot>a \<squnion> ABinds \<Gamma>\<cdot>ae)" by simp
-  also have "Aexp (Let \<Delta> e)\<cdot>a \<squnion> ABinds \<Gamma>\<cdot>ae \<sqsubseteq> ae" using let\<^sub>1 by auto
-  finally
-  have "ABinds (\<Delta> @ \<Gamma>) \<cdot> (Aheap \<Delta> e\<cdot>a \<squnion> ae) \<squnion> Aexp e\<cdot>a \<sqsubseteq> Aheap \<Delta> e\<cdot>a \<squnion> ae"  by this simp
-  }
-  ultimately
-  have "consistent (?ae \<squnion> ae, a) (\<Delta> @ \<Gamma>, e, S) " by auto
-  }
-  moreover
-  {
-    have "\<And> x. x \<in> domA \<Gamma> \<Longrightarrow> x \<notin> edom ?ae"
-      using fresh_distinct[OF let\<^sub>1(1)]
-      by (auto dest!: set_mp[OF edom_Aheap])
-    hence "map_transform Aeta_expand (?ae \<squnion> ae) (map_transform transform (?ae \<squnion> ae) \<Gamma>)
-       = map_transform Aeta_expand ae (map_transform transform ae \<Gamma>)"
-       by (auto intro!: map_transform_cong restrictA_cong simp add: edomIff)
+    have "a_consistent (ae, u, as) ((x,e) # delete x \<Gamma>, e, S)" using lamvar `ae x = up\<cdot>u`
+      by (auto intro!: a_consistent_lamvar simp del: restr_delete)
+    hence "consistent (ae, u, as) ((x, e) # delete x \<Gamma>, e, S)"
+      using lamvar by (auto simp add:  thunks_Cons restr_delete_twist elim: below_trans)
     moreover
 
-    from let\<^sub>1 have *: "edom ae \<subseteq> domA \<Gamma> \<union> upds S" by auto
-    have "\<And> x. x \<in> domA \<Delta> \<Longrightarrow> x \<notin> edom ae"
-       using fresh_distinct[OF let\<^sub>1(1)] fresh_distinct_fv[OF let\<^sub>1(2)] 
-       by (auto dest!: set_mp[OF *] set_mp[OF ups_fv_subset])
-    hence "map_transform Aeta_expand (?ae \<squnion> ae) (map_transform transform (?ae \<squnion> ae) \<Delta>)
-       = map_transform Aeta_expand ?ae (map_transform transform ?ae \<Delta>)"
-       by (auto intro!: map_transform_cong restrictA_cong simp add: edomIff)
+    from `a_consistent _ _`
+    have "Astack (transform_alts as S) \<sqsubseteq> u" by (auto elim: a_consistent_stackD)
+  
+    {
+    from `isVal e`
+    have "isVal (transform u e)" by simp
+    hence "isVal (Aeta_expand u (transform u e))" by (rule isVal_Aeta_expand)
+    moreover
+    from  `map_of \<Gamma> x = Some e`  `ae x = up \<cdot> u`  `isVal (transform u e)`
+    have "map_of (map_transform Aeta_expand ae (map_transform transform ae \<Gamma>)) x = Some (Aeta_expand u (transform u e))"
+      by (simp add: map_of_map_transform)
     ultimately
+    have "a_transform (ae, a, as) (\<Gamma>, Var x, S) \<Rightarrow>\<^sup>*
+          ((x, Aeta_expand u (transform u e)) # delete x (map_transform Aeta_expand ae (map_transform transform ae \<Gamma>)), Aeta_expand u (transform u e), transform_alts as S)"
+       by (auto intro: lambda_var simp del: restr_delete)
+    also have "\<dots> = ((map_transform Aeta_expand ae (map_transform transform ae ((x,e) # delete x \<Gamma>))), Aeta_expand u (transform u e), transform_alts as S)"
+      using `ae x = up \<cdot> u` `isVal (transform u e)`
+      by (simp add: map_transform_Cons map_transform_delete  del: restr_delete)
+    also(subst[rotated]) have "\<dots> \<Rightarrow>\<^sup>* a_transform (ae, u, as) ((x, e) # delete x \<Gamma>, e, S)"
+      by (simp add: restr_delete_twist) (rule Aeta_expand_correct[OF `Astack _ \<sqsubseteq> u`])
+    finally(rtranclp_trans)
+    have "a_transform (ae, a, as) (\<Gamma>, Var x, S) \<Rightarrow>\<^sup>* a_transform (ae, u, as) ((x, e) # delete x \<Gamma>, e, S)".
+    }
+    ultimately show ?case by (blast del: consistentI consistentE)
+  next
+  case (var\<^sub>2 \<Gamma> x e S)
+    have "x \<in> edom ae" using var\<^sub>2 by (auto simp add: a_consistent.simps env_restr_join join_below_iff)
 
-    have "conf_transform (ae, a) (\<Gamma>, Let \<Delta> e, S) \<Rightarrow> conf_transform (?ae \<squnion> ae, a) (\<Delta> @ \<Gamma>, e, S)"
-      using  let\<^sub>1(1,2)
-      by (fastforce intro!: step.intros simp add: map_transform_append  dest: set_mp[OF edom_Aheap])
-  }
-  ultimately
-  show ?case by (blast del: consistentI consistentE)
-next
-  case refl thus ?case by auto
-next
-  case (trans c c' c'')
-    from trans(3)[OF trans(5)]
-    obtain ae' a' where "consistent (ae', a') c'" and *: "conf_transform (ae, a) c \<Rightarrow>\<^sup>* conf_transform (ae', a') c'" by blast
-    from trans(4)[OF this(1)]
-    obtain ae'' a'' where "consistent (ae'', a'') c''" and **: "conf_transform (ae', a') c' \<Rightarrow>\<^sup>* conf_transform (ae'', a'') c''" by blast
-    from this(1) rtranclp_trans[OF * **]
-    show ?case by blast
-qed
+    from var\<^sub>2
+    have "a_consistent (ae, a, as) (\<Gamma>, e, Upd x # S)" by auto
+    from a_consistent_UpdD[OF this  `x \<in> edom ae`]
+    have "ae x = up\<cdot>0" and "a = 0".
 
+    have "a_consistent (ae, a, as) ((x, e) # \<Gamma>, e, S)"
+      using var\<^sub>2 `x \<in> edom ae` by (auto intro!: a_consistent_var\<^sub>2)
+    hence "consistent (ae, 0, as) ((x, e) # \<Gamma>, e, S)"
+      using var\<^sub>2 `a = 0`
+      by (auto simp add: thunks_Cons elim: below_trans)
+    moreover
+    have "a_transform (ae, a, as) (\<Gamma>, e, Upd x # S) \<Rightarrow> a_transform (ae, 0, as) ((x, e) # \<Gamma>, e, S)"
+      using `ae x = up\<cdot>0` `a = 0` var\<^sub>2
+      by (auto intro!: step.intros simp add: map_transform_Cons)
+    ultimately show ?case by (blast del: consistentI consistentE)
+  next
+    case (let\<^sub>1 \<Delta> \<Gamma> e S)
+    let ?ae = "Aheap \<Delta> e\<cdot>a"
+  
+    have "domA \<Delta> \<inter> upds S = {}" using fresh_distinct_fv[OF let\<^sub>1(2)] by (auto dest: set_mp[OF ups_fv_subset])
+    hence *: "\<And> x. x \<in> upds S \<Longrightarrow> x \<notin> edom ?ae" by (auto simp add:  dest!: set_mp[OF edom_Aheap])
+    have restr_stack_simp2: "restr_stack (edom (?ae \<squnion> ae)) S = restr_stack (edom ae) S"
+      by (auto intro: restr_stack_cong dest!: *)
+
+    have "edom ae \<subseteq> domA \<Gamma> \<union> upds S" using let\<^sub>1 by (auto dest!: a_consistent_edom_subsetD)
+    from set_mp[OF this] fresh_distinct[OF let\<^sub>1(1)] fresh_distinct_fv[OF let\<^sub>1(2)]
+    have "edom ae \<inter> domA \<Delta> = {}" by (auto dest: set_mp[OF ups_fv_subset])
+
+    {
+    { fix x e'
+      assume "x \<in> thunks \<Gamma>"
+      with let\<^sub>1
+      have "(?ae \<squnion> ae) x = up\<cdot>0" by auto
+    }
+    moreover
+    { fix x e'
+      assume "x \<in> thunks \<Delta>" 
+      hence "(?ae \<squnion> ae) x = up\<cdot>0" by (auto simp add: Aheap_heap3)
+    }
+    moreover
+    have "heap_upds_ok (\<Gamma>, S)" using let\<^sub>1 by auto
+    with fresh_distinct[OF let\<^sub>1(1)]  `domA \<Delta> \<inter> upds S = {}`
+    have "heap_upds_ok (\<Delta> @ \<Gamma>, S)" by (rule heap_upds_ok_append)
+    moreover
+    
+    have "a_consistent (ae, a, as) (\<Gamma>, Let \<Delta> e, S)"
+      using let\<^sub>1 by auto
+    hence "a_consistent (?ae \<squnion> ae, a, as) (\<Delta> @ \<Gamma>, e, S)"
+      using let\<^sub>1(1,2) `edom ae \<inter> domA \<Delta> = {}` 
+      by (auto intro!:  a_consistent_let simp del: join_comm)
+    ultimately
+    have "consistent (?ae \<squnion> ae, a, as) (\<Delta> @ \<Gamma>, e, S)"
+      by auto
+    }
+    moreover
+    {
+      have "\<And> x. x \<in> domA \<Gamma> \<Longrightarrow> x \<notin> edom ?ae"
+        using fresh_distinct[OF let\<^sub>1(1)]
+        by (auto dest!: set_mp[OF edom_Aheap])
+      hence "map_transform Aeta_expand (?ae \<squnion> ae) (map_transform transform (?ae \<squnion> ae) \<Gamma>)
+         = map_transform Aeta_expand ae (map_transform transform ae \<Gamma>)"
+         by (auto intro!: map_transform_cong restrictA_cong simp add: edomIff)
+      moreover
+  
+      from `edom ae \<subseteq> domA \<Gamma> \<union> upds S`
+      have  "\<And> x. x \<in> domA \<Delta> \<Longrightarrow> x \<notin> edom ae"
+         using fresh_distinct[OF let\<^sub>1(1)] fresh_distinct_fv[OF let\<^sub>1(2)] 
+         by (auto dest!:  set_mp[OF ups_fv_subset])
+      hence "map_transform Aeta_expand (?ae \<squnion> ae) (map_transform transform (?ae \<squnion> ae) \<Delta>)
+         = map_transform Aeta_expand ?ae (map_transform transform ?ae \<Delta>)"
+         by (auto intro!: map_transform_cong restrictA_cong simp add: edomIff)
+      ultimately
+      
+      
+      have "a_transform (ae, a, as) (\<Gamma>, Let \<Delta> e, S) \<Rightarrow> a_transform (?ae \<squnion> ae,  a, as) (\<Delta> @ \<Gamma>, e, S)"
+        using restr_stack_simp2 let\<^sub>1(1,2)
+        apply (auto simp add: map_transform_append restrictA_append  restr_stack_simp2[simplified] map_transform_restrA)
+        apply (rule step.let\<^sub>1)
+        apply (auto dest: set_mp[OF edom_Aheap])
+        done
+    }
+    ultimately
+    show ?case by (blast del: consistentI consistentE)
+  next
+    case (if\<^sub>1 \<Gamma> scrut e1 e2 S)
+    have "consistent (ae, 0, a#as) (\<Gamma>, scrut, Alts e1 e2 # S)"
+      using if\<^sub>1  by (auto dest: a_consistent_if\<^sub>1)
+    moreover
+    have "a_transform (ae,  a, as) (\<Gamma>, scrut ? e1 : e2, S) \<Rightarrow> a_transform (ae, 0, a#as) (\<Gamma>, scrut, Alts e1 e2 # S)"
+      by (auto intro: step.intros)
+    ultimately
+    show ?case by (blast del: consistentI consistentE)
+  next
+    case (if\<^sub>2 \<Gamma> b e1 e2 S)
+    hence "a_consistent (ae, a, as) (\<Gamma>, Bool b, Alts e1 e2 # S)" by auto
+    then  obtain a' as' where [simp]: "as = a' # as'" "a = 0"
+      by (rule a_consistent_alts_on_stack)
+
+    have "consistent (ae, a', as') (\<Gamma>, if b then e1 else e2, S)" 
+      using if\<^sub>2 by (auto dest!: a_consistent_if\<^sub>2)
+    moreover
+    have "a_transform (ae, a, as) (\<Gamma>, Bool b, Alts e1 e2 # S) \<Rightarrow> a_transform (ae,  a', as') (\<Gamma>, if b then e1 else e2, S)"
+      by (auto intro: step.if\<^sub>2[where b = True, simplified] step.if\<^sub>2[where b = False, simplified])
+    ultimately
+    show ?case by (blast del: consistentI consistentE)
+  next
+    case refl thus ?case by auto
+  next
+    case (trans c c' c'')
+      from trans(3)[OF trans(5)]
+      obtain ae' a' as' where "consistent (ae', a', as') c'" and *: "a_transform (ae, a, as) c \<Rightarrow>\<^sup>* a_transform (ae', a', as') c'" by blast
+      from trans(4)[OF this(1)]
+      obtain ae'' a'' as'' where "consistent (ae'', a'', as'') c''" and **: "a_transform (ae', a', as') c' \<Rightarrow>\<^sup>* a_transform (ae'', a'', as'') c''" by blast
+      from this(1) rtranclp_trans[OF * **]
+      show ?case by blast
+  qed
 end
-
 
 end
