Launchbury/Env.thy
@@ -220,6 +220,16 @@ lemma env_delete_env_restr_swap:
   "env_delete x (env_restr S e) = env_restr S (env_delete x e)"
   by (metis (erased, hide_lams) env_delete_def env_restr_fun_upd env_restr_fun_upd_other fun_upd_triv lookup_env_restr_eq)
 
+lemma env_delete_mono:
+  "m \<sqsubseteq> m' \<Longrightarrow> env_delete x m \<sqsubseteq> env_delete x m'"
+  unfolding env_delete_restr
+  by (rule env_restr_mono)
+  
+lemma env_delete_below_arg:
+  "env_delete x m \<sqsubseteq> m"
+  unfolding env_delete_restr
+  by (rule env_restr_below_self)
+
 subsubsection {* Merging of two functions *}
 
 text {*
